Fix admit in case-study/Execute

io/case-study/Execute.fst
@@ -7,7 +7,7 @@ let the_p #a : hist_post #event a = fun lt r -> True
 
 exception Something_went_really_bad
 
-let rec skip_partial_calls (tree:mio int) (_:squash (forall h. dm_mio_theta tree the_p h)) : ML int =
+let rec skip_partial_calls (tree: mio int { forall h. dm_mio_theta tree the_p h }) : ML int =
   match tree with
   | Return y -> y
   | PartialCall pre k -> begin
@@ -15,15 +15,20 @@ let rec skip_partial_calls (tree:mio int) (_:squash (forall h. dm_mio_theta tree
     thus, all asserts are true **)
    assert (dm_mio_theta tree the_p []);
    assert pre;
-   skip_partial_calls (k ()) ()
+   skip_partial_calls (k ())
   end
   (** during extraction, Free.IO.Call is replaced with an actual
   implementation of the commands, therefore, the `Call` constructor
   does not exist **)
   | _ -> raise Something_went_really_bad
 
-let execute (w:unit -> MIO int AllActions (fun _ -> True) (fun _ _ _ -> True)) : ML int =
+open FStar.Tactics
+
+let cast_mio (wp : hist 'a) (t : dm_mio 'a wp) : (x : mio 'a { wp `hist_ord` dm_mio_theta x }) =
+  t
+
+let execute (w:unit -> MIO int AllActions (fun _ -> True) (fun _ _ _ -> True)) : ML int by (compute ()) =
   let dm_tree : dm_gmio int AllActions trivial_hist = reify (w ()) in
   let dm_tree' : dm_mio int trivial_hist = dm_tree in
-  admit ();
-  skip_partial_calls dm_tree' ()
+  let dm_tree2 : (x : mio int { trivial_hist `hist_ord` dm_mio_theta x }) = cast_mio trivial_hist dm_tree' in
+  skip_partial_calls dm_tree2
